examples/gcd_machine.v
@@ -89,14 +89,14 @@ Module GCDMachine.
                      koika_reg_init := init_r;
                      koika_ext_fn_types := empty_Sigma;
                      koika_rules := rules;
+                     koika_rule_external _ := false;
                      koika_scheduler := bring;
                      koika_module_name := "gcd_machine" |};
 
        ip_sim := {| sp_ext_fn_names := empty_fn_names;
                    sp_extfuns := None |};
 
-       ip_verilog := {| vp_ext_fn_names := empty_fn_names;
-                       vp_external_rules := nil |} |}.
+       ip_verilog := {| vp_ext_fn_names := empty_fn_names; |} |}.
 End GCDMachine.
 
 Definition prog := Interop.Backends.register GCDMachine.package.
