tests/extcall.v
@@ -39,8 +39,10 @@ Definition sched : scheduler :=
 Definition sched_result :=
   tc_compute (interp_scheduler (ContextEnv.(create) r) sigma rules sched).
 
+Definition external (r: rule_name_t) := false.
+
 Definition sched_circuits :=
-  compile_scheduler rules sched.
+  compile_scheduler rules external sched.
 
 Definition sched_circuits_result :=
   tc_compute (interp_circuits (ContextEnv.(create) r) sigma sched_circuits).
@@ -53,6 +55,7 @@ Definition package :=
                    koika_reg_init := r;
                    koika_ext_fn_types := Sigma;
                    koika_rules := rules;
+                   koika_rule_external := external;
                    koika_scheduler := sched;
                    koika_module_name := "extcall" |};
 
@@ -64,8 +67,7 @@ public:
   }
 };" |};
 
-     ip_verilog := {| vp_ext_fn_names := verilog_ext_fn_names;
-                     vp_external_rules := [] |} |}.
+     ip_verilog := {| vp_ext_fn_names := verilog_ext_fn_names |} |}.
 
 Definition prog := Interop.Backends.register package.
 Extraction "extcall.ml" prog.
