tests/unpack.v
@@ -58,14 +58,14 @@ Definition package :=
                    koika_reg_init := r;
                    koika_ext_fn_types := empty_Sigma;
                    koika_rules := rules;
+                   koika_rule_external _ := false;
                    koika_scheduler := sched;
                    koika_module_name := "unpack" |};
 
      ip_sim := {| sp_ext_fn_names := empty_fn_names;
                  sp_extfuns := None |};
 
-     ip_verilog := {| vp_ext_fn_names := empty_fn_names;
-                     vp_external_rules := [] |} |}.
+     ip_verilog := {| vp_ext_fn_names := empty_fn_names |} |}.
 
 Definition prog := Interop.Backends.register package.
 Extraction "unpack.ml" prog.
